
### Exercise 1
The identity $(1+x)\sum_{k = 0}^{n}{(-x)^n} = 1 \pm x^{n+1}$ gives an inverse for $n$ large enough. If $a$ is a unit, $a^{-1}x$ is still nilpotent. We just showed that $1+a^{-1}x$ must be a unit, and it follows $a + x$ is a unit. 

### Exercise 2
i) Suppose $f = a_0 + a_1x + \ldots + a_nx^n$ is invertible and nonconstant and let $g = b_0 + b_1x + \ldots + b_mx^m$ be an inverse of $f$, i.e $fg = 1$. 
That means in particular $f(0)g(0) = a_0g(0) = 1$ and $a_0$ is a unit. 
We clearly have $a_n b_m = 0$. 
We also have $a_nb_{m-1} + a_{n-1}b_m = 0$ so  $a_n^2b_{m-1} + a_{n-1}a_nb_m = a_n^2 b_{m-1} = 0$.
Iterating this process we get $a_n^{r+1} b_{m-r} = 0$.
Setting for $r = m$ gives $a_n^{m+1} = 0$ as $b_0$ is a unit. 

Exercise $1$ gives the other implication.

ii) If all the $a_i$ are nilpotent, $f$ is a sum of nilpotents, so it is itself nilpotent.

In the other direction, since $f$ is nilpotent,$\frac{f(x) - f(0)}{x}$ is also nilpotent, because sum of nilpotents is nilpotent and $x$ is regular in $A[x]$. Iterating, we get the result.

iii) Pick $g$ of minimal degree such that $fg = 0$. Since $a_nb_m = 0$, $\deg a_ng < \deg g$ and $a_ngf = 0$ so $a_ng = 0$ by minimality. It follows that $f - a_nx^n$ is still annihilated by $g$, and thus $a_{n-1}b_m = 0$, and then by the same argument $a_{n-1}g = 0$. Iterating, we get $a_kg = 0$ for $0 \leq k \leq n$. This means that $b_m \cdot f = 0$.

iv) Let's denote by $(f)$ the ideal generated by the coefficients of $f$, by abuse of notation. We clearly have $(fg) \subset (f)$ and $(fg) \subset (g)$, which implies that if $fg$ is primitive, $f$ and $g$ are. 
Let's now suppose $f, g$ are primitive and $fg$ is not, and let $I$ be a prime ideal containing $(fg)$. Clearly, $f$ and $g$ are not zero mod $I$, otherwise $1$ would be zero mod $I$, but $fg$ is, contradicting that $I$ is prime.

### Exercise 3
Induction (too lazy to do it properly)

### Exercice 4
Let $f$ be in the Jacobson radical. We will show $f$ is nilpotent. For any $g \in A[X]$, $1 - fg$ is a unit. That means that for any $y \in A$, $1 - f(0)y$